qstar/src/QStarRef.fst
@@ -17,14 +17,14 @@ let pperm = p:perm {p `lesser_equal_perm` full_perm}
 let pts_to (qs:qbits) ([@@@smt_fallback]state:qvec qs) : vprop =
   exists_ (fun (perm:pperm) -> P.pts_to qstar_state ({frac=Some perm; qs; state}))
 
-let apply_gate (#qs:qbits) (#state:qvec qs) (gate:qvec qs -> qvec qs)
+let apply_gate (#qs:qbits) (#state:qvec qs) (g:gate qs)
   : STT unit
     (pts_to qs state)
-    (fun _ -> pts_to qs (gate state))
+    (fun _ -> pts_to qs (apply g state))
   = let perm = elim_exists () in
-    P.upd_gen qstar_state ({frac=Some (Ghost.reveal perm); qs; state}) ({frac=Some (Ghost.reveal perm); qs;state=gate state})
-      (QStarHeap.apply_fpupd #qs #perm #state gate);
-    intro_exists_erased #pperm perm (fun perm -> P.pts_to qstar_state ({frac=Some perm; qs; state=gate state}))
+    P.upd_gen qstar_state ({frac=Some (Ghost.reveal perm); qs; state}) ({frac=Some (Ghost.reveal perm); qs;state=apply g state})
+      (QStarHeap.apply_fpupd #qs #perm #state g);
+    intro_exists_erased #pperm perm (fun perm -> P.pts_to qstar_state ({frac=Some perm; qs; state=apply g state}))
 
 let split_perm (p:pperm)
   : c:pperm{ composable_frac_opt (Some c) (Some c) }
@@ -53,7 +53,6 @@ let share (#o:_) (qs:qbits) (qs':qbits{ disjoint_qbits qs qs'}) (#state:qvec qs)
     intro_pts_to qs ();
     intro_pts_to qs' ()
 
-
 let gather (#o:_) (qs:qbits) (qs':qbits) (#state:qvec qs) (#state':qvec qs')
   : STGhostT (_:unit{ disjoint_qbits qs qs'}) o
     (pts_to qs state `star` pts_to qs' state')
@@ -66,15 +65,6 @@ let gather (#o:_) (qs:qbits) (qs':qbits) (#state:qvec qs) (#state':qvec qs')
             (P.pts_to qstar_state ({frac=Some (sum_perm perm perm'); qs=(qs `OrdSet.union` qs'); state=(state `tensor` state')}));
     intro_pts_to _ ()
 
-
-let project (q:qbit)
-            (qs:qbits {q `OrdSet.mem` qs })
-            (b:bool)
-            (s:qvec qs)
-  : option (qvec (qs `OrdSet.minus` single q))
-  = admit ()
-
-
 [@@warn_on_use "uses an axiom"]
 noextract
 assume //benign; this is defining admit__
@@ -84,13 +74,13 @@ val admit__ (#a:Type)
             (_:unit)
   : STF a p q True (fun _ -> False)
 
-let measure (q:qbit)
-            (qs:qbits { q `OrdSet.mem` qs })
+let measure (#qs:qbits)
+            (q:qbit{ q `OrdSet.mem` qs })
             (state:qvec qs)
-  : STT (b:bool { Some? (project q qs b state) })
+  : STT (b:bool { Some? (proj q b state) })
     (pts_to qs state)
     (fun b -> pts_to (single q) (singleton q b) `star`
-           pts_to (qs `OrdSet.minus` (single q)) (disc q qs b state))
+           pts_to (qs `OrdSet.minus` (single q)) (disc q b state))
   = admit__()
 
 let alloc ()
