qstar/src/QVec.fst
@@ -1,10 +1,7 @@
 module QVec
 
 open FStar.Mul
-//open FStar.Real
-//open Complex
-//open Matrix
-//open Quantum
+open Quantum
 
 module F = FStar.FunctionalExtensionality
 
@@ -29,11 +26,13 @@ let swap_mat : matrix complex 4 4 =
           else if i = 3 && j = 3 then c1
           else c0)
 
-// can we expose this in the OrdSet interface?
+// TODO: can we expose this in the OrdSet interface?
 assume
 val as_list (#a:eqtype) (#f:cmp a) (s:ordset a f) : Tot (l:list a{sorted f l})
 
-// we need some "reorder_indices" function to make the operation commutative
+// Idea: take the normal kronecker product of v0 and v1, and then use repeated
+// applications of swap_mat to reorder qubits so that they correspond to the sorted
+// qubits in qs0 `union` qs1.
 let tensor #qs0 #qs1 v0 v1 = 
   admit()
   //reorder_indices (as_list qs0) (as_list qs1) (kronecker_product v0 v1)
@@ -57,12 +56,66 @@ let tensor_assoc_r #qs0 #qs1 #qs2 v0 v1 v2
             tensor (tensor v0 v1) v2 == tensor v0 (tensor v1 v2))
    = admit()
 
-let init #qs v = admit()
+let proj (#qs:qbits)
+         (q:qbit{q `OrdSet.mem` qs})
+         (b:bool)
+         (s:qvec qs)
+  : option (qvec (qs `OrdSet.minus` single q))
+  = admit()
+    // project qubit q onto state b and check if the result is the zero vector
 
-let disc #qs q v = admit() 
+let disc (#qs:qbits)
+         (q:qbit{q `OrdSet.mem` qs})
+         (b:bool)
+         (s:qvec qs { Some? (proj q b s) })
+  : qvec (qs `OrdSet.minus` single q)
+  = admit()
+    // call proj and then multiply by <b|
 
-let meas #qs q b v = admit() 
+let gate (qs:qbits) = matrix complex (dimension qs) (dimension qs) 
 
-let applyH #qs q v = admit() 
+let hadamard (q:qbit) = hadamard_mat
 
-let applyCX #qs q1 q2 v = admit() 
+let pauli_x (q:qbit) = x_mat
+
+let pauli_z (q:qbit) = z_mat
+
+// 2q gates are a little more complicated than 1q gates because we need to
+// keep in mind the ordering of qubits
+let cnot (q1:qbit) (q2:qbit{q1 <> q2})
+  = if q1 < q2 then cnot_mat
+    else matrix_mul swap_mat (matrix_mul cnot_mat swap_mat)
+
+let apply (#qs:qbits) (g:gate qs) (v:qvec qs) = matrix_mul g v
+
+let lift (qs:qbits) (qs':qbits{qs' `disjoint` qs}) (g:gate qs)
+  = // pad g with identity matrix and then reorder indices
+    admit()
+
+let lift_preserves_frame (qs:qbits) (qs':qbits{qs' `disjoint` qs}) (g:gate qs) 
+                         (v : qvec qs) (v' : qvec qs')
+  : Lemma (ensures (apply (lift qs qs' g) (v `tensor` v') == apply g v `tensor` v'))
+  = admit()
+
+let hadamard_self_adjoint (q:qbit)
+  : Lemma (ensures self_adjoint (hadamard q))
+  = admit()
+
+let pauli_x_self_adjoint (q:qbit)
+  : Lemma (ensures self_adjoint (pauli_x q))
+  = admit()
+
+let pauli_z_self_adjoint (q:qbit)
+  : Lemma (ensures self_adjoint (pauli_z q))
+  = admit()
+
+let cnot_self_adjoint (q1:qbit) (q2:qbit{q1 <> q2})
+  : Lemma (ensures self_adjoint (cnot q1 q2))
+  = admit()
+
+let lemma_bell00 (q1:qbit) (q2:qbit{q1 <> q2}) 
+  : Lemma (apply (cnot q1 q2) 
+                 ((apply (hadamard q1) (singleton q1 false)) `tensor` 
+                    (singleton q2 false))
+           == bell00 q1 q2)
+  = admit()
